# Algebraic Identities

Algebraic identities are equations that hold true for all values of the variables involved. They serve as fundamental tools for simplifying expressions, factoring polynomials, and solving equations efficiently.

---

## Square Identities

### 1. Square of Sum
$$\boxed{(a + b)^2 = a^2 + 2ab + b^2}$$

**Derivation:**
$$
\begin{align*}
(a + b)^2 &= (a + b)(a + b) \\
&= a \cdot a + a \cdot b + b \cdot a + b \cdot b \\
&= a^2 + 2ab + b^2
\end{align*}
$$

**Examples:**
- $(x + 3)^2 = x^2 + 2(x)(3) + 3^2 = x^2 + 6x + 9$
- $(2y + 5)^2 = (2y)^2 + 2(2y)(5) + 5^2 = 4y^2 + 20y + 25$
- $(m + n)^2 = m^2 + 2mn + n^2$

---

### 2. Square of Difference
$$\boxed{(a - b)^2 = a^2 - 2ab + b^2}$$

**Derivation:**
$$
\begin{align*}
(a - b)^2 &= (a - b)(a - b) \\
&= a \cdot a - a \cdot b - b \cdot a + b \cdot b \\
&= a^2 - 2ab + b^2
\end{align*}
$$

**Examples:**
- $(x - 4)^2 = x^2 - 2(x)(4) + 4^2 = x^2 - 8x + 16$
- $(3a - 2)^2 = 9a^2 - 12a + 4$
- $(p - q)^2 = p^2 - 2pq + q^2$

---

### 3. Difference of Squares
$$\boxed{a^2 - b^2 = (a + b)(a - b)}$$

**Derivation:**
$$
\begin{align*}
(a + b)(a - b) &= a \cdot a - a \cdot b + b \cdot a - b \cdot b \\
&= a^2 - b^2
\end{align*}
$$

**Examples:**
- $x^2 - 16 = x^2 - 4^2 = (x + 4)(x - 4)$
- $9y^2 - 25 = (3y)^2 - 5^2 = (3y + 5)(3y - 5)$
- $49 - t^2 = 7^2 - t^2 = (7 + t)(7 - t)$

**Applications:**
- Factoring quadratic expressions
- Simplifying fractions
- Solving equations

---

### 4. Product of Sum and Difference
$$\boxed{(a + b)(a - b) = a^2 - b^2}$$

This is the reverse form of the difference of squares identity.

**Examples:**
- $(x + 5)(x - 5) = x^2 - 25$
- $(2m + 7)(2m - 7) = 4m^2 - 49$
- $(a + b)(a - b) = a^2 - b^2$

---

## Cubic Identities

### 5. Cube of Sum
$$\boxed{(a + b)^3 = a^3 + 3a^2b + 3ab^2 + b^3}$$

**Alternative form:**
$$\boxed{(a + b)^3 = a^3 + b^3 + 3ab(a + b)}$$

**Examples:**
- $(x + 2)^3 = x^3 + 3x^2(2) + 3x(2^2) + 2^3 = x^3 + 6x^2 + 12x + 8$
- $(y + 1)^3 = y^3 + 3y^2 + 3y + 1$
- $(2a + 3)^3 = 8a^3 + 36a^2 + 54a + 27$

---

### 6. Cube of Difference
$$\boxed{(a - b)^3 = a^3 - 3a^2b + 3ab^2 - b^3}$$

**Alternative form:**
$$\boxed{(a - b)^3 = a^3 - b^3 - 3ab(a - b)}$$

**Examples:**
- $(x - 1)^3 = x^3 - 3x^2 + 3x - 1$
- $(2y - 3)^3 = 8y^3 - 36y^2 + 54y - 27$
- $(m - n)^3 = m^3 - 3m^2n + 3mn^2 - n^3$

---

### 7. Sum of Cubes
$$\boxed{a^3 + b^3 = (a + b)(a^2 - ab + b^2)}$$

**Derivation:**
$$
\begin{align*}
(a + b)(a^2 - ab + b^2) &= a^3 - a^2b + ab^2 + a^2b - ab^2 + b^3 \\
&= a^3 + b^3
\end{align*}
$$

**Examples:**
- $x^3 + 8 = x^3 + 2^3 = (x + 2)(x^2 - 2x + 4)$
- $27y^3 + 1 = (3y)^3 + 1^3 = (3y + 1)(9y^2 - 3y + 1)$
- $a^3 + 64 = a^3 + 4^3 = (a + 4)(a^2 - 4a + 16)$

---

### 8. Difference of Cubes
$$\boxed{a^3 - b^3 = (a - b)(a^2 + ab + b^2)}$$

**Derivation:**
$$
\begin{align*}
(a - b)(a^2 + ab + b^2) &= a^3 + a^2b + ab^2 - a^2b - ab^2 - b^3 \\
&= a^3 - b^3
\end{align*}
$$

**Examples:**
- $x^3 - 27 = x^3 - 3^3 = (x - 3)(x^2 + 3x + 9)$
- $8m^3 - 1 = (2m)^3 - 1^3 = (2m - 1)(4m^2 + 2m + 1)$
- $125 - n^3 = 5^3 - n^3 = (5 - n)(25 + 5n + n^2)$

---

## Multi-Term Identities

### 9. Square of Trinomial
$$\boxed{(a + b + c)^2 = a^2 + b^2 + c^2 + 2ab + 2ac + 2bc}$$

**Derivation:**
$$
\begin{align*}
(a + b + c)^2 &= [(a + b) + c]^2 \\
&= (a + b)^2 + 2(a + b)c + c^2 \\
&= a^2 + 2ab + b^2 + 2ac + 2bc + c^2 \\
&= a^2 + b^2 + c^2 + 2ab + 2ac + 2bc
\end{align*}
$$

**Examples:**
- $(x + y + 2)^2 = x^2 + y^2 + 4 + 2xy + 4x + 4y$
- $(a + b + c)^2 = a^2 + b^2 + c^2 + 2ab + 2ac + 2bc$
- $(1 + 2 + 3)^2 = 1 + 4 + 9 + 4 + 6 + 12 = 36 = 6^2$ âœ“

---

### 10. Sum of Squares (Important Relation)
$$\boxed{a^2 + b^2 = (a + b)^2 - 2ab}$$
$$\boxed{a^2 + b^2 = (a - b)^2 + 2ab}$$

**Examples:**
- $x^2 + 9 = (x + 3)^2 - 6x$ or $(x - 3)^2 + 6x$

---

## Additional Useful Identities

### 11. Four Terms Identity
$$\boxed{(a + b)(c + d) = ac + ad + bc + bd}$$

**Example:**
- $(x + 2)(y + 3) = xy + 3x + 2y + 6$

---

### 12. Sophie Germain Identity
$$\boxed{a^4 + 4b^4 = (a^2 + 2b^2 + 2ab)(a^2 + 2b^2 - 2ab)}$$

**Application:** Factoring certain fourth-degree polynomials.

---

## Quick Reference Table

| Identity | Formula |
|----------|---------|
| Square of Sum | $(a + b)^2 = a^2 + 2ab + b^2$ |
| Square of Difference | $(a - b)^2 = a^2 - 2ab + b^2$ |
| Difference of Squares | $a^2 - b^2 = (a + b)(a - b)$ |
| Cube of Sum | $(a + b)^3 = a^3 + 3a^2b + 3ab^2 + b^3$ |
| Cube of Difference | $(a - b)^3 = a^3 - 3a^2b + 3ab^2 - b^3$ |
| Sum of Cubes | $a^3 + b^3 = (a + b)(a^2 - ab + b^2)$ |
| Difference of Cubes | $a^3 - b^3 = (a - b)(a^2 + ab + b^2)$ |

---

## Practice Tips

1. **Memorize the patterns**: Recognize the structure of each identity
2. **Practice substitution**: Try various values for $a$ and $b$ to verify
3. **Factor first**: Look for common factors before applying identities
4. **Work backwards**: Practice both expanding and factoring
5. **Combine identities**: Some problems require multiple identities

---

## See Also
- [[Binomials]] - Binomial theorem and expansion
- [[Polynomials]] - Polynomial operations and factoring
- [[Quadratic Function]] - Applications of square identities
- [[00 - Algebra MOC]] - Algebra topics overview
